

Answer Key and Marking Scheme

Q1 Answer

- (1) We need to prove 3 properties of distance metric

Property 1: $d(x, y) \geq 0$ as $d(x, y)$ involves taking sum of non-negative numbers due to the use of $|\cdot|$, $\sum_{i=1}^n |x_i - y_i|$ can be zero only when each component of form $x_i - y_i = 0$. This only happens when $x = y$. Hence $d(x, y) = 0$ only for $x = y$. (0.5 marks)

Property 2: Since $|x_i - y_i| = |y_i - x_i|$, it can be concluded that $d(x, y) = d(y, x)$. (0.5 marks)

Property 3: Note $d(x, y) = \sum_{i=1}^n |x_i - y_i| = \sum_{i=1}^n |x_i - z_i + z_i - y_i|$. Now using triangle inequality of ℓ_1 norm.

$$\sum_{i=1}^n |x_i - z_i + z_i - y_i| \leq \sum_{i=1}^n |x_i - z_i| + \sum_{i=1}^n |z_i - y_i| = d(x, z) + d(z, y)$$

Hence $d(x, y) \leq d(x, z) + d(z, y)$. (1 marks)

In summary $d(x, y)$ is a distance metric.

- (2) $\cos^2(\theta) = \frac{(x_1^T A x_2)^2}{(x_1^T A x_1)(x_2^T A x_2)}$. Substitute values given in question to get

$$\cos^2(\theta) = \frac{(37+26\alpha)^2}{(5\alpha^2+12\alpha+9)(154)} \quad (1 \text{ marks})$$

(i) $\cos(45^\circ) = \frac{1}{\sqrt{2}}$. The previous equation after substitution of θ can be rearranged to get $291\alpha^2 + 1000\alpha + 676 = 0$ (0.5 marks)

Finally solution by quadratic formula is $\alpha = \frac{-1000 \pm \sqrt{1000^2 - 4 \cdot 291 \cdot 676}}{2 \cdot 291}$

(ii) $\cos(0^\circ) = 1$. The previous equation after substitution of θ can be rearranged to get $94\alpha^2 - 76\alpha + 17 = 0$ (0.5 marks)

Finally solution by quadratic formula is $\alpha = \frac{76 \pm \sqrt{76^2 - 4 \cdot 94 \cdot 17}}{2 \cdot 94}$. Observe that here α do not have real solution.

NOTE: Give 0.5 marks in the previous 2 steps if the student has written correctly upto the quadratic equation in each case. The final step in two subparts using quadratic formula is not compulsory

- (3) a) Recall that $\det(C_1) = \text{Product of its eigenvalues}$. Since 0 is one of its eigenvalues, hence $\det(C_1) = 0$ (0.5 marks).

Since $\det(C_1) = \det(AB) = \det(A) \cdot \det(B) = \det(B) \cdot \det(A) = \det(BA) = \det(C_2)$. Hence $\det(C_2) = 0$. This means 0 is one of eigenvalues of C_2 as determinant is product of eigenvalues. (0.5 marks)

- b) $G = PA$. Recall that $A = U\Sigma V^T$. So $G = PU\Sigma V^T$.

Now since P, U are orthogonal matrices $P^{-1} = P^T$ and $U^{-1} = U^T$. This means $(PU)^T = U^T P^T = U^{-1} P^{-1} = (PU)^{-1}$. Hence PU is orthogonal matrix. (0.25 marks)

Hence SVD of G is $(PU)\Sigma V^T$ (0.25 marks)

$E = AP$. Recall that $A = U\Sigma V^T$. So $E = U\Sigma V^T P$.

Now since P, V are orthogonal matrices $P^{-1} = P^T$ and $V^{-1} =$

V^T . This means $(V^T P)^T = P^T V = P^{-1}(V^{-1})^T = P^{-1}(V^T)^{-1} = (V^T P)^{-1}$. Hence $V^T P$ is orthogonal matrix. (0.25 marks)

Hence SVD of E is $U\Sigma(V^T P)$ (0.25 marks)

(4) Taking partial derivatives we get $\frac{\partial f}{\partial x} = 2x + 3y$, $\frac{\partial f}{\partial y} = 3x + 3y^2$.

Now taking derivatives of functions $x(r)$ and $y(r)$ with respect to r we get $\frac{dx}{dr} = -\sin(r)$ and $\frac{dy}{dr} = \cos(r)$. (0.5 marks)

Now using chain rule

$$\frac{df}{dr} = \frac{\partial f}{\partial x} \frac{dx}{dr} + \frac{\partial f}{\partial y} \frac{dy}{dr} = (2x + 3y)(-\sin(r)) + (3x + 3y^2)(\cos(r))$$

(0.25 marks)

Now substituting definition of $x(r)$ and $y(r)$, we get

$$\frac{df}{dr} = (2\cos(r) + 3\sin(r))(-\sin(r)) + (3\cos(r) + 3(\sin(r))^2)(\cos(r))$$

Finally, simplifying we get

$$\frac{df}{dr} = -2\sin(r)\cos(r) - 3\sin^2(r) + 3\cos^2(r) + 3\sin^2(r)\cos(r)$$

(0.25 marks)

Q2

1) $f(\mathbf{X}) = \mathbf{a}^T \mathbf{X} \mathbf{a}$

i. Clearly, using identity, $\frac{\partial f}{\partial \mathbf{X}} = \mathbf{a} \mathbf{a}^T$. (1 mark)

ii. If \mathbf{a} is a zero vector, then $\frac{\partial f}{\partial \mathbf{X}}$ is zero matrix and hence of rank 0.

Therefore rank 1 approximation doesnot exist. (1 mark)

If \mathbf{a} is a nonzero vector, then there exist $a_i \neq 0$.

$$\text{Then } \frac{\partial f}{\partial \mathbf{X}} = \mathbf{a} \mathbf{a}^T = \begin{bmatrix} a_1 \mathbf{a}^T \\ \vdots \\ a_i \mathbf{a}^T \\ \vdots \\ a_{1000} \mathbf{a}^T \end{bmatrix}.$$

$$\text{Now } R_j - \frac{a_j}{a_i} R_i, \forall j = 1, \dots, 1000 \text{ and } j \neq i, \text{ will give } \begin{bmatrix} \mathbf{0}^T \\ \vdots \\ a_i \mathbf{a}^T \\ \vdots \\ \mathbf{0}^T \end{bmatrix}.$$

By interchanging i^{th} and 1^{st} row we get $\begin{bmatrix} a_i \mathbf{a}^T \\ \mathbf{0}^T \\ \vdots \\ \mathbf{0}^T \end{bmatrix}$, which is REF and

hence $\frac{\partial f}{\partial \mathbf{X}} = \mathbf{a} \mathbf{a}^T$ is rank 1 matrix. (2 marks)

Therefore, the rank 1 approximation exists and is the same as the actual matrix. (1 mark)

2) Now $f : \mathbb{R}^4 \rightarrow \mathbb{R}$ is defined as

$$f(\mathbf{x}) = [x_1, x_2, x_3, x_4] \begin{bmatrix} 1 & 3 & 2 & 2 \\ 2 & 6 & 4 & 2 \\ 3 & 3 & 0 & 2 \\ 0 & 1 & 1 & 2 \end{bmatrix} \begin{bmatrix} x_1 \\ x_2 \\ x_3 \\ x_4 \end{bmatrix} = \mathbf{x}^T \begin{bmatrix} 1 & 3 & 2 & 2 \\ 2 & 6 & 4 & 2 \\ 3 & 3 & 0 & 2 \\ 0 & 1 & 1 & 2 \end{bmatrix} \mathbf{x} \text{ when } \mathbf{x} = \begin{bmatrix} x_1 \\ x_2 \\ x_3 \\ x_4 \end{bmatrix}.$$

$$\begin{aligned} \text{i. } \nabla_{\mathbf{x}} f(\mathbf{x}) &= \frac{\partial f}{\partial \mathbf{x}} = \mathbf{x}^T \left(\begin{bmatrix} 1 & 3 & 2 & 2 \\ 2 & 6 & 4 & 2 \\ 3 & 3 & 0 & 2 \\ 0 & 1 & 1 & 2 \end{bmatrix} + \begin{bmatrix} 1 & 2 & 3 & 0 \\ 3 & 6 & 3 & 1 \\ 2 & 4 & 0 & 1 \\ 2 & 2 & 2 & 2 \end{bmatrix} \right) \\ \Rightarrow \nabla_{\mathbf{x}} f(\mathbf{x}) &= \mathbf{x}^T \begin{pmatrix} \begin{bmatrix} 2 & 5 & 5 & 2 \\ 5 & 12 & 7 & 3 \\ 5 & 7 & 0 & 3 \\ 2 & 3 & 3 & 4 \end{bmatrix} \end{pmatrix} \end{aligned} \quad (1 \text{ mark})$$

$$\text{ii. } \nabla_{\mathbf{x}} f(\mathbf{x}) = \mathbf{0}^T$$

$$\begin{aligned} \Rightarrow \mathbf{x}^T \begin{pmatrix} \begin{bmatrix} 2 & 5 & 5 & 2 \\ 5 & 12 & 7 & 3 \\ 5 & 7 & 0 & 3 \\ 2 & 3 & 3 & 4 \end{bmatrix} \end{pmatrix} &= \mathbf{0}^T \\ \Rightarrow \begin{bmatrix} 2 & 5 & 5 & 2 \\ 5 & 12 & 7 & 3 \\ 5 & 7 & 0 & 3 \\ 2 & 3 & 3 & 4 \end{bmatrix} \mathbf{x} &= \mathbf{0} \end{aligned}$$

To solve this, we will convert coefficient matrix into REF which is equal to

$$\begin{bmatrix} 2 & 5 & 5 & 2 \\ 0 & -0.5 & -5.5 & -2 \\ 0 & 0 & 48 & 20 \\ 0 & 0 & 0 & 5/3 \end{bmatrix}$$

The rank of the matrix is 4 and the number of variables is also 4. Therefore, the solution is unique and the unique solution is $[0, 0, 0, 0]^T$. (2 marks)

Q3

a We see that when the transform \mathbf{A} is applied four times, it results in the input vector itself. So, this can be rotation by 90° in the counter clockwise direction. (2 marks)

$$\begin{aligned} \text{So, } \mathbf{A} &= \begin{bmatrix} \cos(90^\circ) & -\sin(90^\circ) \\ \sin(90^\circ) & \cos(90^\circ) \end{bmatrix} \\ &= \begin{bmatrix} 0 & -1 \\ 1 & 0 \end{bmatrix} \end{aligned} \quad (2 \text{ marks})$$

b For the matrix \mathbf{A} , eigen values are:

$$\lambda_1 = i, \lambda_2 = -i \quad (1 \text{ mark})$$

eigen vector corresponding to eigen value $\lambda_1 = i$ is $[i, 1]^T$

eigen vector corresponding to eigen value $\lambda_2 = -i$ is $[-i, 1]^T$ (1 mark)

c \mathbf{A} is rotation in counter clockwise. Hence, \mathbf{A}^{-1} will be rotation in clockwise direction. (1 mark)

Yes, $(\mathbf{A}^{-1})^4$ will also be I , as applying 90° clockwise rotation successively to a vector 4 times gives back the same vector. (1 mark)

Q4

(1) (a) $\dim(V) = \frac{n(n+1)}{2}$ (1.5 marks)

(b) $\dim(W) = \frac{n(n+1)}{2}$ (1.5 marks)

(2) $\mathbf{k} = \begin{bmatrix} -2 \\ 0 \\ 0 \end{bmatrix}$ (1.25 marks)

$$R = \begin{bmatrix} 1 & -0.5 & 2.5 \\ 0 & 0 & 0 \\ 0 & 0 & 0 \end{bmatrix} \quad (2.75 \text{ marks})$$